theories/refinements/static_gradual/compat_cast/between_rec.v
@@ -1,18 +1,19 @@
-From fae_gtlc_mu.refinements.static_gradual Require Export logical_relation resources_right compat_easy help_left compat_cast.defs.
+From fae_gtlc_mu.refinements.static_gradual Require Export logical_relation resources_right compat_easy help_left compat_cast.defs tactics_left.
 From fae_gtlc_mu.cast_calculus Require Export types typing.
-From fae_gtlc_mu.stlc_mu Require Export lang.
 From fae_gtlc_mu.cast_calculus Require Export lang.
 From iris.algebra Require Import list.
 From iris.proofmode Require Import tactics.
 From iris.program_logic Require Import lifting.
-From fae_gtlc_mu.cast_calculus Require Export types.
 From fae_gtlc_mu.cast_calculus Require Export consistency.structural.definition.
 From fae_gtlc_mu.backtranslation Require Export cast_help.general cast_help.extract cast_help.embed.
-
+From fae_gtlc_mu.cast_calculus Require Export lang types.
+(* From iris.program_logic Require Import language. *)
 (* Coercion stlc_mu.lang.of_val : stlc_mu.lang.val >-> stlc_mu.lang.expr. *)
 (* Coercion cast_calculus.lang.of_val : cast_calculus.lang.val >-> cast_calculus.lang.expr. *)
 
 (* Notation "# v" := (of_val v) (at level 20). *)
+
+(* Coercion of_val : val >-> expr. *)
 
 Section between_rec.
   Context `{!heapG Σ,!gradRN Σ}.
@@ -30,12 +31,6 @@ Section between_rec.
 
   (* Lemma compat_cast_between_TRec A τl τr (p : (TRec τl, TRec τr) ∉ A) (pC : cons_struct ((TRec τl, TRec τr) :: A) ). *)
 
-
-  Definition back_cast_ar {A} {τi τf} (pC : cons_struct A τi τf) :=
-  ∀ ei' K' v v' fs, bi_entails
-                      (rel_cast_functions A fs ∗ interp τi [] (v, v') ∗ initially_inv ei' ∗ currently_half (fill K' (Cast (# v') τi τf)))
-                      (WP (𝓕c pC fs (stlc_mu.lang.of_val v)) {{ w, ∃ w', currently_half (fill K' (# w')) ∗ interp τf [] (w, w') }})%I.
-
   (** Proving it *)
 
   Lemma refold_interp_unknown' vv' : fixpoint interp_unknown1' vv' ≡ interp TUnknown [] vv'.
@@ -43,297 +38,167 @@ Section between_rec.
     auto.
   Qed.
 
-  (* Lemma back_cast_ar_all {A} {τi τf} (pC : cons_struct A τi τf) : back_cast_ar pC. *)
-  (* Proof. *)
-  (*   induction pC; rewrite /𝓕c /𝓕 /back_cast_ar; iIntros (ei' K' v v' fs) "(Hfs & #Hvv' & #Hei' & Hv')". *)
-  (*   - rewrite /𝓕c /𝓕 extract_no_subs. *)
-  (*     destruct G. *)
-  (*     + (** TUnit *) rewrite unfold_fixpoint_interp_unknown1'. *)
-  (*       iDestruct "Hvv'" as "[Hvv'Unit|[Hpp'|[Hss'|[Hff'|Huu']]]]". *)
-  (*       * iDestruct "Hvv'Unit" as "%"; inversion H; clear v v' H H1 H2. *)
-  (*         admit. *)
-  (*       * iDestruct "Hpp'" as (v1 v1' v2 v2') "(% & #H1 & #H2)". simpl in H; inversion H; clear H H1 H2 v v'. *)
-  (*         repeat rewrite (refold_interp_unknown'). *)
-  (*         admit. *)
-  (*       * iDestruct "Hss'" as "[H1 | H2]". *)
-  (*         -- iDestruct "H1" as (v1 v1') "[% Hv1v1']"; rewrite (refold_interp_unknown'); inversion H; clear H H1 H2 v v'. *)
-  (*            admit. *)
-  (*         -- iDestruct "H2" as (v2 v2') "[% Hv2v2']"; rewrite (refold_interp_unknown'); inversion H; clear H H1 H2 v v'. *)
-  (*            admit. *)
-  (*       * iDestruct "Hff'" as (f f') "[% Hff']". inversion H. clear H H1 H2 v v'. *)
-  (*         admit. *)
-  (*       * iDestruct "Huu'" as (u u') "[% H]"; rewrite (refold_interp_unknown'); inversion H; clear H H1 H2 v v'. *)
-  (*         admit. *)
-  (*       * constructor. *)
-  (*     + (** TProd *) admit. *)
-  (*     + (** TSum *) admit. *)
-  (*     + (** TArrow *) rewrite unfold_fixpoint_interp_unknown1'. *)
-  (*       iDestruct "Hvv'" as "[Hvv'Unit|[Hpp'|[Hss'|[Hff'|Huu']]] ]". *)
-  (*       * iDestruct "Hvv'Unit" as "%"; inversion H; clear v v' H H1 H2. *)
-  (*         admit. *)
-  (*       * iDestruct "Hpp'" as (v1 v1' v2 v2') "(% & #H1 & #H2)". simpl in H; inversion H; clear H H1 H2 v v'. *)
-  (*         repeat rewrite (refold_interp_unknown'). *)
-  (*         admit. *)
-  (*       * iDestruct "Hss'" as "[H1 | H2]". *)
-  (*         -- iDestruct "H1" as (v1 v1') "[% Hv1v1']"; rewrite (refold_interp_unknown'); inversion H; clear H H1 H2 v v'. *)
-  (*            admit. *)
-  (*         -- iDestruct "H2" as (v2 v2') "[% Hv2v2']"; rewrite (refold_interp_unknown'); inversion H; clear H H1 H2 v v'. *)
-  (*            admit. *)
-  (*       * iDestruct "Hff'" as (f f') "[% Hff']". inversion H. clear H H1 H2 v v'. *)
-  (*         admit. *)
-  (*       * iDestruct "Huu'" as (u u') "[% H]"; rewrite (refold_interp_unknown'); inversion H; clear H H1 H2 v v'. *)
-  (*         admit. *)
-  (*       * constructor. *)
-  (*     + (** TRec *) rewrite unfold_fixpoint_interp_unknown1'. *)
-  (*       iDestruct "Hvv'" as "[Hvv'Unit|[Hpp'|[Hss'|[Hff'|Huu']]] ]". *)
-  (*       * iDestruct "Hvv'Unit" as "%"; inversion H; clear v v' H H1 H2. *)
-  (*         admit. *)
-  (*       * iDestruct "Hpp'" as (v1 v1' v2 v2') "(% & #H1 & #H2)". simpl in H; inversion H; clear H H1 H2 v v'. *)
-  (*         repeat rewrite (refold_interp_unknown'). *)
-  (*         admit. *)
-  (*       * iDestruct "Hss'" as "[H1 | H2]". *)
-  (*         -- iDestruct "H1" as (v1 v1') "[% Hv1v1']"; rewrite (refold_interp_unknown'); inversion H; clear H H1 H2 v v'. *)
-  (*            admit. *)
-  (*         -- iDestruct "H2" as (v2 v2') "[% Hv2v2']"; rewrite (refold_interp_unknown'); inversion H; clear H H1 H2 v v'. *)
-  (*            admit. *)
-  (*       * iDestruct "Hff'" as (f f') "[% Hff']". inversion H. clear H H1 H2 v v'. *)
-  (*         admit. *)
-  (*       * iDestruct "Huu'" as (u u') "[% H]"; rewrite (refold_interp_unknown'); inversion H; clear H H1 H2 v v'. *)
-  (*         admit. *)
-  (*       * constructor. *)
-  (*   - rewrite /𝓕c /𝓕. rewrite embed_no_subs. destruct G. *)
-  (*     + iDestruct "Hvv'" as "%". simpl in H. inversion H. rewrite H0 H1. clear v v' H H0 H1. *)
-  (*       admit. *)
-  (*     + iDestruct "Hvv'" as ((v1 , v1') (v2 , v2')) "[% [H1 H2]]". simpl in H; inversion H; clear H H1 H2 v v'. *)
-  (*       admit. *)
-  (*     + iDestruct "Hvv'" as "[H1 | H2]". *)
-  (*       * iDestruct "H1" as ((v1 , v1')) "[% H1]". *)
-  (*         simpl in H; inversion H; clear H H1 H2 v v'. *)
-  (*         admit. *)
-  (*       * iDestruct "H2" as ((v2 , v2')) "[% H2]". *)
-  (*         simpl in H; inversion H; clear H H1 H2 v v'. *)
-  (*         admit. *)
-  (*     + admit. *)
-  (*     + admit. *)
-  (*   - admit. *)
-  (*   - admit. *)
-  (*   - admit. *)
-  (*   - admit. *)
-  (*   - admit. *)
-  (*   - admit. *)
-  (*   - fold interp. simpl. admit. *)
-  (*   - rewrite /𝓕c /𝓕. *)
-  (*     fold (𝓕 pC). simpl. *)
-  (*     (* asimpl. fold between_TRec. (𝓕c pC2 fs). *) *)
-  (*     admit. *)
-  (*   - admit. *)
+  Lemma back_cast_ar_trec_trec_use:
+    ∀ (A : list (type * type)) (τl τr : {bind type}) (i : nat) (pμτlμtrinA : A !! i = Some (TRec τl, TRec τr)),
+      back_cast_ar (consTRecTRecUseCall A τl τr i pμτlμtrinA).
+  Proof.
+    intros A τl τr i pμτlμtr.
+    rewrite /𝓕c /𝓕 /back_cast_ar; iIntros (ei' K' v v' fs) "(#Hfs & #Hvv' & #Hei' & Hv')".
+    rewrite /𝓕c /𝓕. asimpl.
+    (** getting the information about the length of the list *)
+    iDestruct "Hfs" as "[% Hfs']".
+    (* iAssert (rel_cast_functions A fs) with "[Hfs']" as "Hfs". iSplit; done. *)
+    destruct (fs !! i) as [f | abs] eqn:Hf.
+    rewrite (stlc_mu.typing.env_subst_lookup _ i f); try done.
+    {
+      iDestruct (big_sepL2_lookup with "Hfs'") as "#Hf". exact pμτlμtr. exact Hf.
+      iApply ("Hf" $! v v' with "Hvv'"). done.
+    }
+    { (* trivially impossible case *)
+      assert (Hi : i < length fs). rewrite -H. by eapply lookup_lt_Some.
+      assert (Hi' : i >= length fs). by apply lookup_ge_None_1. exfalso. lia.
+    }
+  Qed.
 
-  (* Admitted. *)
+  Lemma wp_fix'' (f : stlc_mu.lang.expr) Φ :
+    ⊢ (▷ ▷ WP f (stlc_mu.lang.Lam (rename (+1) (Fix'' f) (stlc_mu.lang.Var 0)))   {{ Φ }} -∗ (WP (Fix'' f) {{ Φ }}))%I.
+  Proof.
+    iIntros "H".
+    rewrite{2} /Fix''.
+    iApply (wp_bind $ stlc_mu.lang.fill_item $ stlc_mu.lang.AppLCtx _).
+    apply (@ectxi_lang_ctx_item stlc_mu.lang.ectxi_lang). (* hmmmm :( *)
+    wp_head.
+    (* iApply wp_pure_step_later; auto; iNext. *)
+    iApply wp_value.
+    simpl.
+    iApply wp_pure_step_later; auto; iNext.
+    asimpl.
+    iApply "H".
+  Qed.
 
 
+  Lemma back_cast_ar_trec_trec_expose:
+    ∀ (A : list (type * type)) (τl τr : {bind type}) (pμτlμτrnotA : (TRec τl, TRec τr) ∉ A)
+      (pC : ((TRec τl, TRec τr) :: A) ⊢ τl.[TRec τl/] ~ τr.[TRec τr/]) (IHpC : back_cast_ar pC),
+      back_cast_ar (consTRecTRecExposeCall A τl τr pμτlμτrnotA pC).
+  Proof.
+    intros A τl τr pμτlμτrnotA pC IHpC.
+    rewrite /𝓕c /𝓕 /back_cast_ar; iIntros (ei' K' v v' fs) "(#Hfs & #Hvv' & #Hei' & Hv')".
+    (** setting up iLöb *)
+    iLöb as "IHlob" forall (v v' ei' K') "Hvv' Hei'".
+    fold (𝓕c (consTRecTRecExposeCall A τl τr pμτlμτrnotA pC) fs).
+    (* iRevert (ei' K' v v') "Hvv' Hei' Hv'". *)
+    rewrite {2}/𝓕c. rewrite /𝓕.
+    fold (𝓕 pC).
+    (** rewriting value relation for v and v' *)
+    rewrite fixpoint_interp_rec1_eq.
+    iDestruct "Hvv'" as ([w w']) "#[% Hww']".
+    inversion H; clear v v' H H1 H2.
+    fold interp.
+    fold (interp_rec ⟦ τl ⟧ []).
+    assert (bydef : interp_rec ⟦ τl ⟧ [] = ⟦ TRec τl ⟧ []); auto; rewrite bydef. clear bydef.
+    rewrite (interp_subst [] τl (TRec τl) (w, w')).
+    (** evaluation steps in WP *)
+    (* applying to value v *)
+    iApply wp_pure_step_later; auto; iNext.
+    (* bringing subs of fs inwards *)
+    rewrite rewrite_subs_app.
+    do 2 rewrite Fix''_subs_rewrite.
+    assert (triv :
+              Fix'' (stlc_mu.lang.Lam (stlc_mu.lang.Lam (stlc_mu.lang.Fold (rename (+1) (𝓕 pC).[upn 1 (ren (+1))] (stlc_mu.lang.Unfold (stlc_mu.lang.Var 0)))))).[up (stlc_mu.typing.env_subst fs)].[stlc_mu.lang.of_val $ stlc_mu.lang.FoldV w/] (stlc_mu.lang.Var 0).[up (stlc_mu.typing.env_subst fs)].[stlc_mu.lang.of_val $ stlc_mu.lang.FoldV w/] = Fix'' (stlc_mu.lang.Lam (stlc_mu.lang.Lam (stlc_mu.lang.Fold ((𝓕 pC).[up (stlc_mu.typing.env_subst fs) >> ren (+1)] (stlc_mu.lang.Unfold (ids 0)))))) (stlc_mu.lang.Fold (w))). by asimpl. rewrite triv. clear triv.
+    (* evaluation step of the Fix'' itself *)
+    iApply (wp_bind (stlc_mu.lang.fill_item $ stlc_mu.lang.AppLCtx _)).
+    iApply wp_fix''.
+    (** easy steps *)
+    iApply wp_pure_step_later; auto; iNext.
+    do 2 iNext.
+    iApply wp_value.
+    iApply wp_pure_step_later; auto; iNext. (* unfold fold w *)
+    (** rewriting *)
 
+    assert (triv : ((stlc_mu.lang.Fold ((𝓕 pC).[up (stlc_mu.typing.env_subst fs) >> ren (+1)] (stlc_mu.lang.Unfold (ids 0)))).[up
+                                                                                                                (stlc_mu.lang.Lam
+                                                                                                                    (rename (+1)
+                                                                                                                      (Fix''
+                                                                                                                          (stlc_mu.lang.Lam
+                                                                                                                            (stlc_mu.lang.Lam
+                                                                                                                                (stlc_mu.lang.Fold
+                                                                                                                                  ((𝓕 pC).[up
+                                                                                                                                        (stlc_mu.typing.env_subst fs) >>
+                                                                                                                                      ren (+1)]
+                                                                                                                                      (stlc_mu.lang.Unfold (ids 0)))))))
+                                                                                                                      (stlc_mu.lang.Var 0)) .: ids)].[stlc_mu.lang.Fold ( w)/]) = (stlc_mu.lang.Fold ((𝓕 pC).[(between_TRec' (𝓕 pC)).[stlc_mu.typing.env_subst fs] .: stlc_mu.typing.env_subst fs] (stlc_mu.lang.Unfold (stlc_mu.lang.Fold (w)))))).
 
-
-
-  (*       fold interp_unknown1 interp_unknown. *)
-  (*       rewrite interp_unknown_unfold /interp_unknown1; iDestruct "Hvv'" as "#Hvv'"; iDestruct "Hvv'" as "[Hvv'Unit|[Hpp'|[Hss'|[Hff'|Hur']]] ]"; fold interp_unknown1 interp_unknown. *)
-  (*       * iDestruct "Hvv'Unit" as ((w , w')) "[% Hww']"; simpl in H; inversion H; clear v v' H H1 H2. *)
-  (*         asimpl. *)
-  (*         iApply wp_pure_step_later; auto; iNext; asimpl. *)
-  (*         iDestruct "Hww'" as "%"; inversion H; rewrite H0 H1; clear w w' H H0 H1. *)
-  (*         iApply (wp_bind (stlc_mu.lang.fill_item $ stlc_mu.lang.CaseCtx _ _)). *)
-  (*         iApply wp_pure_step_later; auto; iNext. *)
-  (*         iApply wp_value. *)
-  (*         iApply wp_pure_step_later; auto; iNext. *)
-  (*         iApply wp_pure_step_later; auto; iNext. asimpl. *)
-  (*         iApply wp_pure_step_later; auto; iNext. *)
-  (*         iApply wp_pure_step_later; auto; iNext. asimpl. *)
-  (*         iMod (step_pure _ ei' K' (Cast (Cast Unit TUnit ⋆) ⋆ TUnit) (# UnitV) with "[Hv']") as "HHHH"; intros; auto. *)
-  (*         apply Same_Ground with (v := UnitV ); auto; constructor. *)
-  (*         iApply wp_value. *)
-  (*         iExists UnitV. *)
-  (*         by repeat iFrame. *)
-  (*       * (* diverging branch *) *)
-  (*         iDestruct "Hpp'" as ((p , p')) "[% Hpp']"; simpl in H; inversion H; clear H H1 H2 v v'. *)
-  (*         asimpl. *)
-  (*         iApply wp_pure_step_later; auto; iNext; asimpl. *)
-  (*         iDestruct "Hpp'" as ((v1 , v1') (v2 , v2')) "[% [Hv1v1' Hv2v2']]"; simpl in H; inversion H; clear H H1 H2 p p'. *)
-  (*         iApply (wp_bind (stlc_mu.lang.fill_item $ stlc_mu.lang.CaseCtx _ _)). *)
-  (*         iApply wp_pure_step_later; auto; iNext. *)
-  (*         iApply wp_value. *)
-  (*         iApply wp_pure_step_later; auto; iNext; asimpl. *)
-  (*         iApply wp_pure_step_later; auto; iNext; asimpl. *)
-  (*         iApply wp_pure_step_later; auto; iNext. asimpl. *)
-  (*         by iApply wp_Ω. *)
-  (*       * admit. *)
-  (*       * admit. *)
-  (*       * iDestruct "Hur'" as ((u , r')) "[% Hr]". simpl in H. inversion H. clear H H1 H2. *)
-  (*         admit. *)
-  (*     + rewrite interp_unknown_unfold /interp_unknown1; iDestruct "Hvv'" as "#Hvv'"; iDestruct "Hvv'" as "[Hvv'Unit|[Hpp'|[Hss'|[Hff'|Hur']]] ]"; fold interp_unknown1 interp_unknown. *)
-  (*       * (* diverging branch *) *)
-  (*         iDestruct "Hvv'Unit" as ((w , w')) "[% Hww']"; simpl in H; inversion H; clear v v' H H1 H2. *)
-  (*         asimpl. *)
-  (*         iApply wp_pure_step_later; auto; iNext; asimpl. *)
-  (*         iDestruct "Hww'" as "%"; inversion H; rewrite H0 H1; clear w w' H H0 H1. *)
-  (*         iApply (wp_bind (stlc_mu.lang.fill_item $ stlc_mu.lang.CaseCtx _ _)). *)
-  (*         iApply wp_pure_step_later; auto; iNext. *)
-  (*         iApply wp_value. *)
-  (*         iApply (wp_bind (stlc_mu.lang.fill_item $ stlc_mu.lang.CaseCtx _ _)). *)
-  (*         iApply wp_value. *)
-  (*         iApply wp_pure_step_later; auto; iNext. *)
-  (*         iApply wp_pure_step_later; auto; iNext. asimpl. *)
-  (*         iApply wp_pure_step_later; auto; iNext. asimpl. *)
-  (*         by iApply wp_Ω. *)
-  (*       * iDestruct "Hpp'" as ((p , p')) "[% Hpp']"; simpl in H; inversion H; clear H H1 H2. *)
-  (*         asimpl. *)
-  (*         iApply wp_pure_step_later; auto; iNext; asimpl. *)
-  (*         iDestruct "Hpp'" as ((v1 , v1') (v2 , v2')) "[% [Hv1v1' Hv2v2']]"; simpl in H; inversion H; clear H H1 H2 p p'. *)
-  (*         iApply (wp_bind (stlc_mu.lang.fill_item $ stlc_mu.lang.CaseCtx _ _)). *)
-  (*         iApply wp_pure_step_later; auto; iNext. *)
-  (*         iApply wp_value. *)
-  (*         iApply wp_pure_step_later; auto; iNext; asimpl. *)
-  (*         iApply wp_pure_step_later; auto; iNext; asimpl. *)
-  (*         iApply wp_pure_step_later; auto; iNext. asimpl. *)
-  (*         iMod (step_pure _ ei' K' *)
-  (*                         (Cast *)
-  (*                            (Cast (Pair (# v1') (# v2')) *)
-  (*                                  (⋆ × ⋆) ⋆) ⋆ *)
-  (*                            (⋆ × ⋆) *)
-  (*                         ) *)
-  (*                         (Pair (# v1') (# v2')) *)
-  (*                 with "[Hv']") as "HHHH"; auto. *)
-  (*         intro. eapply Same_Ground. simplify_option_eq. auto. constructor. *)
-  (*         iApply wp_value. *)
-  (*         iExists (PairV (v1') (v2')). *)
-  (*         simpl. repeat iFrame. *)
-  (*         iExists (v1 , v1') , (v2 , v2'). by auto. *)
-  (*       * admit. *)
-  (*       * admit. *)
-  (*       * admit. *)
-  (*     + admit. *)
-  (*     + admit. *)
-  (*     + rewrite interp_unknown_unfold /interp_unknown1; iDestruct "Hvv'" as "#Hvv'"; iDestruct "Hvv'" as "[Hvv'Unit|[Hpp'|[Hss'|[Hff'|Hur']]] ]"; fold interp_unknown1 interp_unknown. *)
-  (*       * admit. *)
-  (*       * admit. *)
-  (*       * admit. *)
-  (*       * admit. *)
-  (*       * iDestruct "Hur'" as ((u , r')) "[% Hur']"; inversion H; clear H H1 H2. *)
-  (*         iMod (step_pure _ ei' K' *)
-  (*                         (Cast (# castupV_TRec r') ⋆ (TRec ⋆)) *)
-  (*                         (# r') *)
-  (*                 with "[Hv']") as "HHHH"; auto. *)
-  (*         intro; eapply Same_Ground; simplify_option_eq; auto; constructor. *)
-  (*         iApply wp_pure_step_later; auto; iNext; asimpl. *)
-  (*         iApply (wp_bind (stlc_mu.lang.fill_item $ stlc_mu.lang.CaseCtx _ _)). *)
-  (*         iApply wp_pure_step_later; auto. *)
-  (*         iApply wp_value. simpl.  *)
-  (*         iApply wp_pure_step_later; auto. asimpl.  *)
-  (*         iApply wp_value. *)
-  (*         repeat iNext. *)
-  (*         iExists r'. by iFrame. *)
-  (*   - destruct G; rewrite /𝓕c /𝓕. *)
-  (*     + iApply wp_pure_step_later; auto; iNext; asimpl. *)
-  (*       iDestruct "Hvv'" as "%"; inversion H. rewrite H0 H1. clear H H0 H1 v v'. *)
-  (*       iApply wp_value. iExists (CastV UnitV TUnit ⋆ (From_ground_to_unknown TUnit Ground_TUnit)). *)
-  (*       simpl in *. *)
-  (*       iFrame. *)
-  (*       rewrite interp_unknown_unfold /interp_unknown1. *)
-  (*       admit. *)
-  (*     + admit. *)
-  (*     + admit. *)
-  (*     + admit. *)
-  (*     + rewrite fixpoint_interp_rec1_eq. *)
-  (*       iDestruct "Hvv'" as ((r , r')) "[% #Hrr']". inversion H; clear H H1 H2. *)
-  (*       iApply wp_pure_step_later; auto; iNext; asimpl. *)
-  (*       iApply (wp_bind (fill [stlc_mu.lang.InjRCtx ; stlc_mu.lang.FoldCtx ])). *)
-  (*       iApply wp_pure_step_later; auto. iNext; asimpl. *)
-  (*       iApply wp_value. *)
-  (*       iApply wp_value. *)
-  (*       iExists (CastV (FoldV r') (TRec ⋆) ⋆ (From_ground_to_unknown (TRec ⋆) Ground_TRec)). *)
-  (*       simpl in *. *)
-  (*       iFrame. *)
-  (*       rewrite{1} interp_unknown_unfold. *)
-  (*       rewrite{1} interp_unknown_unfold. *)
-  (*       repeat rewrite{1} /interp_unknown1. *)
-  (*       iRight. *)
-  (*       iRight. *)
-  (*       iRight. *)
-  (*       iRight. *)
-  (*       iModIntro. *)
-  (*       iExists (r , FoldV r'). simpl. iSplitL. *)
-  (*       auto. *)
-  (*       admit. *)
-  (*   - admit. *)
-  (*   - admit. *)
-  (*   - rewrite /𝓕c /𝓕. asimpl. *)
-  (*     iApply wp_pure_step_later; auto. *)
-  (*     asimpl. *)
-  (*     iDestruct "Hvv'" as %[eq1 eq2]; simplify_eq. *)
-  (*     iNext. *)
-  (*     iMod (step_pure _ ei' K' (Cast (# UnitV) TUnit TUnit) (# UnitV) with "[Hv']") as "HHHH"; auto. *)
-  (*     intros; by eapply IdBase. *)
-  (*     iApply wp_value. *)
-  (*     iExists UnitV. iFrame. iSplit; trivial. *)
-  (*   - rewrite /𝓕c /𝓕; asimpl. *)
-  (*     iMod (step_pure _ ei' K' (Cast (# v') ⋆ ⋆) (# v') with "[Hv']") as "Hv'"; auto. *)
-  (*     intros; by eapply IdStar. *)
-  (*     iApply wp_pure_step_later; auto; asimpl. *)
-  (*     iNext. *)
-  (*     iApply wp_value. *)
-  (*     iExists v'. iFrame. *)
-  (*   - iDestruct "Hvv'" as "[Hvv'1 | Hvv'2]". *)
-  (*     + iDestruct "Hvv'1" as (vv'1) "Hvv'1". destruct vv'1 as (v1 , v1'). *)
-  (*       iDestruct "Hvv'1" as "[% Hvv'1]". inversion H. *)
-  (*       iMod (step_pure _ ei' K' (Cast (# InjLV v1') (τ1 + τ2)%type (τ1' + τ2')%type) _ with "[Hv']") as "Hv'"; auto; try (intros; eapply SumCast; auto). *)
-  (*       iMod ((step_case_inl _ ei' K' (# v1')) with "[Hv']") as "Hv'"; auto. *)
-  (*       (* rewrite /𝓕c /𝓕 /between_TSum. *) *)
-  (*       rewrite /𝓕c /𝓕. *)
-  (*       iApply wp_pure_step_later. auto; asimpl. *)
-  (*       iApply wp_pure_step_later; auto; asimpl. *)
-  (*       iNext. iNext. *)
-  (*       iApply wp_bind. admit. *)
-  (*       iApply wp_wand_r. *)
-  (*       iSplitL. *)
-  (*       iApply (IHpC1 ei' (InjLCtx :: K')). repeat iFrame. auto. *)
-  (*       clear H H1 H2 v1 v1'. *)
-  (*       iIntros (v1) "HHH". iDestruct "HHH" as (v1') "[Hv1' Hvv'1]". *)
-  (*       iApply wp_value. *)
-  (*       iExists (InjLV v1'). repeat iFrame. iLeft. iExists (v1 , v1'). *)
-  (*       iSplitR. by simpl. done. *)
-  (*     + admit. *)
-  (*   - iSimpl in "Hvv'". iDestruct "Hvv'" as ((v1 , v1') (v2 , v2')) "[% [Hv1v1' Hv2v2']]". simpl in H; inversion H; clear H H1 H2 v v'. *)
-  (*     iApply wp_pure_step_later; auto. *)
-  (*     fold (𝓕 pC1) (𝓕 pC2). asimpl. fold (𝓕c pC1 fs) (𝓕c pC2 fs). *)
-  (*     iDestruct "Hfs" as "[% Hfs']"; iAssert (rel_cast_functions A fs) with "[Hfs']" as "Hfs". iSplit; done. *)
-  (*     rewrite 𝓕c_rewrite. *)
-  (*     iApply (wp_bind (fill [stlc_mu.lang.AppRCtx (𝓕cV pC1 fs H) ; stlc_mu.lang.PairLCtx ((𝓕c pC2 fs) (stlc_mu.lang.Snd (stlc_mu.lang.Pair (stlc_mu.lang.of_val v1) (stlc_mu.lang.of_val v2)))) ])). *)
-  (*     iApply wp_pure_step_later; auto. *)
-  (*     do 2 iNext. iApply wp_value. simpl. *)
-  (*     iApply (wp_bind (fill [stlc_mu.lang.PairLCtx ((𝓕c pC2 fs) (stlc_mu.lang.Snd (stlc_mu.lang.Pair (stlc_mu.lang.of_val v1) (stlc_mu.lang.of_val v2)))) ])). *)
-  (*     rewrite -𝓕c_rewrite. *)
-  (*     iApply (wp_wand with "[Hfs Hv1v1' Hei' Hv']"). *)
-  (*     (* iApply (IHpC1 ei' :: K' with "Hfs Hv1v1' Hei' Hv'"). *) *)
-  (*     admit. *)
-  (*     admit. *)
-  (*   - admit. *)
-  (*   - rewrite /𝓕c /𝓕. *)
-  (*     fold (𝓕 pC). *)
-  (*     iApply wp_pure_step_later; auto; asimpl. *)
-  (*     iApply (wp_bind $ stlc_mu.lang.fill_item $ stlc_mu.lang.AppLCtx _). *)
-  (*     iApply wp_pure_step_later; auto; asimpl. *)
-  (*     iApply wp_pure_step_later; auto; asimpl. *)
-
-  (*   - rewrite /𝓕c /𝓕. asimpl. *)
-  (*     destruct (fs !! i) as [f | abs] eqn:Hf. *)
-  (*     + rewrite (stlc_mu.typing.env_subst_lookup _ _ f); auto. *)
-  (*       iDestruct "Hfs" as "[% Hfs]". *)
-  (*       rewrite fixpoint_interp_rec1_eq. *)
-        
-  (*       rewrite interp_unknown_unfold /interp_unknown1. *)
-  (*       unfold fixpoint_re *)
-  (*       iAssert  *)
-        
-  (*   destruct () *)
+    by asimpl. rewrite triv. clear triv.
+    rewrite between_TRec'_subst_rewrite.
+    rewrite between_TRec'_to_value.
+    assert (H : (𝓕 pC).[stlc_mu.lang.of_val (between_TRecV' (𝓕 pC).[up (stlc_mu.typing.env_subst fs)]) .: stlc_mu.typing.env_subst fs] = (𝓕 pC).[stlc_mu.typing.env_subst (between_TRecV' (𝓕 pC).[up (stlc_mu.typing.env_subst fs)] :: fs)]); first by simpl. rewrite H; clear H.
+    (** easy steps *)
+    iApply (wp_bind (stlc_mu.lang.fill_item $ stlc_mu.lang.FoldCtx)).
+    iDestruct "Hfs" as "[% Hfs']"; iAssert (rel_cast_functions A fs) with "[Hfs']" as "Hfs". iSplit; done.
+    (* iDestruct "Hfs" as "[% Hfs]". *)
+    assert (Hs : length ((TRec τl, TRec τr) :: A) =
+                length
+                  (between_TRecV'
+                      (𝓕 pC).[up (stlc_mu.typing.env_subst fs)] :: fs)). simpl; auto.
+    fold (𝓕c pC (between_TRecV' (𝓕 pC).[up (stlc_mu.typing.env_subst fs)] :: fs)).
+    (* fold (𝓕c (consTRecTRecExposeCall A τl τr pμτlμτrnotA pC) fs). *)
+    rewrite (𝓕c_rewrite pC).
+    iApply (wp_bind (stlc_mu.lang.fill_item $ stlc_mu.lang.AppRCtx _)).
+    iApply wp_pure_step_later; auto; iNext.
+    iApply wp_value.
+    fold (𝓕c (consTRecTRecExposeCall A τl τr pμτlμτrnotA pC) fs).
+    simpl. (** hmmm; unfolds IHLöb... *)
+    (** rewriting stuff *)
+    rewrite -(𝓕c_rewrite pC) {2}/𝓕c.
+    assert (T : between_TRecV' (𝓕 pC).[up (stlc_mu.typing.env_subst fs)] =
+                (𝓕cV (consTRecTRecExposeCall A τl τr pμτlμτrnotA pC) fs H)
+            ). {
+      apply stlc_mu.lang.of_val_inj.
+      rewrite -between_TRec'_to_value.
+      rewrite -between_TRec'_subst_rewrite.
+      by simpl.
+      (* rewrite -𝓕c_rewrite. rewrite /𝓕c. *)
+      (* by simpl. *)
+    } rewrite T. clear T.
+    (** eval specification side *)
+    iMod (step_pure _ ei' K'
+                    (Cast (Fold w') (TRec τl) (TRec τr))
+                    (Fold (Cast (Unfold (Fold w')) (τl.[TRec τl/]) (τr.[TRec τr/]))) with "[Hv']") as "Hv'".
+    intros. apply (RecursiveCast _ (FoldV w')). by rewrite -to_of_val. auto. by iFrame.
+    iMod (step_pure _ ei' (CastCtx τl.[TRec τl/] τr.[TRec τr/] :: FoldCtx :: K')
+                    (Unfold (Fold (# w')))
+                    w' with "[Hv']") as "Hv'".
+    intros. apply (Unfold_Fold _ w'). by rewrite to_of_val. auto. by iFrame.
+    (** apply IH *)
+    iApply (wp_wand with "[-]").
+    iApply (IHpC ei' (FoldCtx :: K') w w' (𝓕cV (consTRecTRecExposeCall A τl τr pμτlμτrnotA pC) fs H :: fs)). iSplitL "Hfs". iSplitR; first by done.
+    (* iApply (IHpC ei' (FoldCtx :: K') w w' (𝓕cV (consTRecTRecExposeCall A τl τr pμτlμτrnotA pC) fs H :: fs)). iSplitL "Hfs". iSplitR; first by done. *)
+    (** applying IHlob and Hfs *)
+    (* rewrite /𝓕c. *)
+    iSplit.
+    iModIntro. iIntros (v v') "#Hvv'".
+    { clear K'. iIntros (K') "Hv'". iSimpl in "Hv'".
+      rewrite -𝓕c_rewrite.
+      iApply ("IHlob" $! v v' with "Hv' Hvv' Hei'").
+    }
+    done.
+    (** other *)
+    iSplitR. done. iSplitR. done. by simpl.
+    (** finish *)
+    iIntros (v) "H".
+    iDestruct "H" as (v') "[Hv' #Hvv']".
+    iApply wp_value.
+    iExists (FoldV v').
+    iFrame.
+    rewrite fixpoint_interp_rec1_eq.
+    simpl. iModIntro.
+    iExists (v , v').
+    iSplitR. done.
+    iNext.
+    by rewrite (interp_subst [] τr (TRec τr) (v, v')).
+    (* trival shells here *)
+  Admitted.
 
 
 End between_rec.
