theories/backtranslation/cast_help/factorize.v
@@ -1,4 +1,4 @@
-From fae_gtlc_mu.cast_calculus Require Export types consistency.structural.definition.
+From fae_gtlc_mu.cast_calculus Require Export types.
 From fae_gtlc_mu.stlc_mu Require Export typing lang lib.fix.
 From fae_gtlc_mu.backtranslation.cast_help Require Export universe embed extract.
 
@@ -20,6 +20,12 @@ Definition factorization_up (f : expr) (τG : cast_calculus.types.type) (G : Gro
       embed τG G ((rename (+1) f) (Var 0))
     ).
 
+Lemma factorization_up_subst_rewrite (f : expr) (τG : cast_calculus.types.type) (G : Ground τG) σ : (factorization_up f τG G).[σ] = factorization_up f.[σ] τG G.
+Proof.
+  rewrite /factorization_up.
+  asimpl. by rewrite embed_no_subs.
+Qed.
+
 Lemma factorization_up_typed Γ {f : expr} (τ : type(* backtranslation of something that is not a ground type, nor star *)) (τG : cast_calculus.types.type) (G : Ground τG) (d : Γ ⊢ₛ f : (TArrow τ <<τG>>)) :
   Γ ⊢ₛ factorization_up f τG G : (TArrow τ Universe).
 Proof.
@@ -35,6 +41,12 @@ Definition factorization_down (f : expr) (τG : cast_calculus.types.type) (G : G
   Lam (
       (rename (+1) f) (extract τG G (Var 0))
     ).
+
+Lemma factorization_down_subst_rewrite (f : expr) (τG : cast_calculus.types.type) (G : Ground τG) σ : (factorization_down f τG G).[σ] = factorization_down f.[σ] τG G.
+Proof.
+  rewrite /factorization_down.
+  asimpl. by rewrite extract_no_subs.
+Qed.
 
 Lemma factorization_down_typed Γ {f : expr} (τ : type(* backtranslation of something that is not a ground type, nor star *)) (τG : cast_calculus.types.type) (G : Ground τG) (d : Γ ⊢ₛ f : (TArrow <<τG>> τ)) :
   Γ ⊢ₛ factorization_down f τG G : (TArrow Universe τ).
