theories/cast_calculus/consistency/standard.v
@@ -2,29 +2,26 @@ From Autosubst Require Export Autosubst.
 From fae_gtlc_mu Require Import prelude cast_calculus.types.
 Require Coq.Logic.JMeq.
 
-Reserved Notation "n |> τ ~ τ'" (at level 4, τ, τ' at next level).
-Inductive cons_stand : nat -> type -> type -> Type :=
-| GenSymUnit n : cons_stand n TUnit TUnit
-| GenSymUnknownL n (τ : type) : (UB n τ) -> cons_stand n ⋆ τ
-| GenSymUnknownR n (τ : type) : (UB n τ) -> cons_stand n τ ⋆
-| GenSymSum n
+Inductive cons_stand : type -> type -> Type :=
+| GenSymUnit : cons_stand TUnit TUnit
+| GenSymUnknownL (τ : type) : cons_stand ⋆ τ
+| GenSymUnknownR (τ : type) : cons_stand τ ⋆
+| GenSymSum
     (τ1 τ1' τ2 τ2' : type)
-    (s1 : cons_stand n τ1 τ1')
-    (s2 : cons_stand n τ2 τ2')
-  : cons_stand n (τ1 + τ2)%type (τ1' + τ2')%type
-| GenSymProd n
+    (s1 : cons_stand τ1 τ1')
+    (s2 : cons_stand τ2 τ2')
+  : cons_stand (τ1 + τ2)%type (τ1' + τ2')%type
+| GenSymProd
     (τ1 τ1' τ2 τ2' : type)
-    (s1 : cons_stand n τ1 τ1')
-    (s2 : cons_stand n τ2 τ2')
-  : cons_stand n (τ1 × τ2) (τ1' × τ2')
-| GenSymArrow n
+    (s1 : cons_stand τ1 τ1')
+    (s2 : cons_stand τ2 τ2')
+  : cons_stand (τ1 × τ2) (τ1' × τ2')
+| GenSymArrow
     (τ1 τ1' τ2 τ2' : type)
-    (s1 : cons_stand n τ1 τ1')
-    (s2 : cons_stand n τ2 τ2')
-  : cons_stand n (TArrow τ1 τ2) (TArrow τ1' τ2')
-| GenSymVar n (i : nat) :
-    i < n ->
-    cons_stand n (TVar i) (TVar i)
-| GenSymRec n (τ τ' : type) (P : cons_stand (S n) τ τ') :
-    cons_stand n (TRec τ) (TRec τ')
-where "n |> τ ~ τ'" := (cons_stand n τ τ').
+    (s1 : cons_stand τ1 τ1')
+    (s2 : cons_stand τ2 τ2')
+  : cons_stand (TArrow τ1 τ2) (TArrow τ1' τ2')
+| GenSymVar (i : nat) :
+    cons_stand (TVar i) (TVar i)
+| GenSymRec (τ τ' : type) (P : cons_stand τ τ') :
+    cons_stand (TRec τ) (TRec τ').
